formal/Syntax.v
@@ -10,8 +10,11 @@
     - Mutable variable assignment (set)
     - Sequential composition and while loops
     - Lambda abstractions and function application
-    - Array literals, indexing, and length
-    - Record (struct) literals and field access
+    - Recursive functions (fix)
+    - Array literals, indexing, length, update, and push
+    - Record (struct) literals, field access, and field update
+    - Variant types and pattern matching
+    - String indexing
 *)
 
 From Stdlib Require Import ZArith.
@@ -23,13 +26,14 @@ Open Scope string_scope.
 (** ** Types *)
 
 Inductive ty : Type :=
-  | TInt    : ty                    (* int *)
-  | TBool   : ty                    (* bool *)
-  | TString : ty                    (* string *)
-  | TUnit   : ty                    (* unit *)
-  | TArrow  : ty -> ty -> ty        (* function type: T1 -> T2 *)
-  | TArray  : ty -> ty              (* array type: array<T> *)
-  | TRecord : list (string * ty) -> ty.  (* record type: {f1: T1, ..., fn: Tn} *)
+  | TInt     : ty                             (* int *)
+  | TBool    : ty                             (* bool *)
+  | TString  : ty                             (* string *)
+  | TUnit    : ty                             (* unit *)
+  | TArrow   : ty -> ty -> ty                 (* function type: T1 -> T2 *)
+  | TArray   : ty -> ty                       (* array type: array<T> *)
+  | TRecord  : list (string * ty) -> ty       (* record type: {f1: T1, ..., fn: Tn} *)
+  | TVariant : list (string * ty) -> ty.      (* variant type: Tag1(T1) | ... | Tagn(Tn) *)
 
 (** ** Binary operators *)
 
@@ -64,24 +68,31 @@ Inductive unop : Type :=
 (** ** Expressions *)
 
 Inductive expr : Type :=
-  | EInt    : Z -> expr                         (* integer literal *)
-  | EBool   : bool -> expr                      (* boolean literal *)
-  | EString : string -> expr                    (* string literal *)
-  | EUnit   : expr                              (* unit literal *)
-  | EVar    : string -> expr                     (* variable reference *)
-  | EBinOp  : binop -> expr -> expr -> expr      (* binary operation *)
-  | EUnOp   : unop -> expr -> expr               (* unary operation *)
-  | EIf     : expr -> expr -> expr -> expr       (* if cond then e1 else e2 *)
-  | ELet    : string -> expr -> expr -> expr     (* let x = e1 in e2 *)
-  | ESet    : string -> expr -> expr             (* set x = e *)
-  | ESeq    : expr -> expr -> expr               (* e1; e2 *)
-  | EWhile  : expr -> expr -> expr               (* while cond do body *)
-  | ELam    : string -> ty -> expr -> expr       (* fun (x : T) => body *)
-  | EApp    : expr -> expr -> expr               (* function application *)
-  | EArray  : list expr -> expr                  (* array literal: [e1, ..., en] *)
-  | EIndex  : expr -> expr -> expr               (* array indexing: (at arr i) *)
-  | ERecord : list (string * expr) -> expr       (* record literal: {f1: e1, ..., fn: en} *)
-  | EField  : expr -> string -> expr.            (* field access: e.f *)
+  | EInt       : Z -> expr                              (* integer literal *)
+  | EBool      : bool -> expr                           (* boolean literal *)
+  | EString    : string -> expr                         (* string literal *)
+  | EUnit      : expr                                   (* unit literal *)
+  | EVar       : string -> expr                         (* variable reference *)
+  | EBinOp     : binop -> expr -> expr -> expr          (* binary operation *)
+  | EUnOp      : unop -> expr -> expr                   (* unary operation *)
+  | EIf        : expr -> expr -> expr -> expr           (* if cond then e1 else e2 *)
+  | ELet       : string -> expr -> expr -> expr         (* let x = e1 in e2 *)
+  | ESet       : string -> expr -> expr                 (* set x = e *)
+  | ESeq       : expr -> expr -> expr                   (* e1; e2 *)
+  | EWhile     : expr -> expr -> expr                   (* while cond do body *)
+  | ELam       : string -> ty -> expr -> expr           (* fun (x : T) => body *)
+  | EApp       : expr -> expr -> expr                   (* function application *)
+  | EFix       : string -> string -> ty -> ty -> expr -> expr  (* fix f (x:T1):T2 = body *)
+  | EArray     : list expr -> expr                      (* array literal: [e1, ..., en] *)
+  | EIndex     : expr -> expr -> expr                   (* array indexing: (at arr i) *)
+  | EArraySet  : expr -> expr -> expr -> expr           (* functional array update *)
+  | EArrayPush : expr -> expr -> expr                   (* array push (append) *)
+  | ERecord    : list (string * expr) -> expr           (* record literal *)
+  | EField     : expr -> string -> expr                 (* field access: e.f *)
+  | ESetField  : string -> string -> expr -> expr       (* set x.f = e *)
+  | EConstruct : string -> expr -> ty -> expr           (* variant constructor: Tag(e) : T *)
+  | EMatch     : expr -> list (string * string * expr) -> expr  (* match e { Tag x => body, ... } *)
+  | EStrIndex  : expr -> expr -> expr.                  (* string indexing: s[i] *)
 
 (** ** Values
 
@@ -89,13 +100,15 @@ Inductive expr : Type :=
     that cannot be reduced further. *)
 
 Inductive val : Type :=
-  | VInt    : Z -> val                           (* integer value *)
-  | VBool   : bool -> val                        (* boolean value *)
-  | VString : string -> val                      (* string value *)
-  | VUnit   : val                                (* unit value *)
-  | VClos   : string -> expr -> env -> val       (* closure: param, body, captured env *)
-  | VArray  : list val -> val                    (* array value *)
-  | VRecord : list (string * val) -> val         (* record value *)
+  | VInt       : Z -> val                               (* integer value *)
+  | VBool      : bool -> val                            (* boolean value *)
+  | VString    : string -> val                          (* string value *)
+  | VUnit      : val                                    (* unit value *)
+  | VClos      : string -> expr -> env -> val           (* closure: param, body, captured env *)
+  | VFixClos   : string -> string -> expr -> env -> val (* fix closure: f, x, body, captured env *)
+  | VArray     : list val -> val                        (* array value *)
+  | VRecord    : list (string * val) -> val             (* record value *)
+  | VConstruct : string -> val -> val                   (* variant value: tag, payload *)
 
 (** ** Environments
 
@@ -129,7 +142,7 @@ Fixpoint env_update (x : string) (v : val) (e : env) : env :=
     else ECons y v' (env_update x v rest)
   end.
 
-(** ** Association list lookup (polymorphic) *)
+(** ** Association list operations (polymorphic) *)
 
 Fixpoint assoc_lookup {A : Type} (x : string) (l : list (string * A)) : option A :=
   match l with
@@ -137,12 +150,42 @@ Fixpoint assoc_lookup {A : Type} (x : string) (l : list (string * A)) : option A
   | (y, v) :: rest => if String.eqb x y then Some v else assoc_lookup x rest
   end.
 
+Fixpoint assoc_update {A : Type} (x : string) (v : A) (l : list (string * A)) : list (string * A) :=
+  match l with
+  | [] => []
+  | (y, v') :: rest =>
+    if String.eqb x y then (y, v) :: rest
+    else (y, v') :: assoc_update x v rest
+  end.
+
+(** ** List update (functional) *)
+
+Fixpoint list_update {A : Type} (n : nat) (v : A) (l : list A) : list A :=
+  match l with
+  | [] => []
+  | x :: rest =>
+    match n with
+    | 0 => v :: rest
+    | S n' => x :: list_update n' v rest
+    end
+  end.
+
+(** ** Branch lookup for pattern matching *)
+
+Fixpoint find_branch (tag : string) (branches : list (string * string * expr)) : option (string * expr) :=
+  match branches with
+  | [] => None
+  | (t, x, body) :: rest =>
+    if String.eqb tag t then Some (x, body)
+    else find_branch tag rest
+  end.
+
 (** ** Type equality decidability *)
 
 Lemma ty_eq_dec : forall (t1 t2 : ty), {t1 = t2} + {t1 <> t2}.
 Proof.
   fix IH 1.
-  intros [| | | | ta tb | ta | fs1] [| | | | ta' tb' | ta' | fs2];
+  intros [| | | | ta tb | ta | fs1 | vs1] [| | | | ta' tb' | ta' | fs2 | vs2];
     try (left; reflexivity); try (right; discriminate).
   - (* TArrow *)
     destruct (IH ta ta'); [| right; congruence].
@@ -162,6 +205,18 @@ Proof.
     + destruct (string_dec s1 s2); [subst | right; congruence].
       destruct (IH t1 t2); [subst | right; congruence].
       destruct (IHfs fs2'); [subst | right; congruence].
+      left; reflexivity.
+  - (* TVariant *)
+    enough ({vs1 = vs2} + {vs1 <> vs2}) as [->|];
+      [left; reflexivity | right; congruence |].
+    revert vs2.
+    induction vs1 as [|[s1 t1] vs1' IHvs]; intros [|[s2 t2] vs2'].
+    + left; reflexivity.
+    + right; discriminate.
+    + right; discriminate.
+    + destruct (string_dec s1 s2); [subst | right; congruence].
+      destruct (IH t1 t2); [subst | right; congruence].
+      destruct (IHvs vs2'); [subst | right; congruence].
       left; reflexivity.
 Defined.
 
